New Features: 1) reading argc argv envp of the main function from the standard input 2) changed      id = malloc typ sz align    to be      id = malloc typ value align
   The size to malloc can be anything with type i32, for example, constant, constant expression, or value

Fix a bug:

Designed a constant expression folding in OCaml, because the LLVM interface to GEP needs indices to be constants, in the case they are constant expressions, we should explicitly fold them to be constants.

Known problems to fix:

1) recursive types
2) LLVM intrinsic function
3) some cases run very slow, the implementation of algorithm operations could be a problem
4) instructions: extractelement, metadata, switch, invoke



git-svn-id: https://webdav.seas.upenn.edu/svn/sol/vol@2716 eef5ea85-cc2e-0410-bd84-0fae1f012da8

src/Parser/coq2llvm.ml
@@ -30,7 +30,7 @@ let rec translate_typ (ctx:llcontext) (ty:LLVMsyntax.typ) : lltype =
 let rec translate_constant (ctx:llcontext) (c:LLVMsyntax.const) : llvalue = 
 	match c with
   | LLVMsyntax.Coq_const_zeroinitializer t ->  Llvm.const_null (translate_typ ctx t)
-	| LLVMsyntax.Coq_const_int (sz, i) -> Llvm.APInt.const_apint (Llvm.global_context()) i
+	| LLVMsyntax.Coq_const_int (sz, i) -> Llvm.APInt.const_apint ctx i
 	| LLVMsyntax.Coq_const_floatpoint (fp, f) -> Llvm.APFloat.const_apfloat ctx f
 	| LLVMsyntax.Coq_const_undef t -> undef (translate_typ ctx t)
 	| LLVMsyntax.Coq_const_null t ->  const_null (translate_typ ctx t)
