src/TV/symexe_dec.v
@@ -67,13 +67,13 @@ Proof.
     destruct st2; try solve [done_right].
     destruct (@H s1); subst; try solve [done_right].
     destruct (@typ_dec t t0); subst; try solve [done_right].
-    destruct (@Size.dec s0 s2); subst; try solve [done_right].
+    destruct (@H0 st2); subst; try solve [done_right].
     destruct (@Align.dec a a0); subst; try solve [auto | done_right].
   Case "sterm_alloca".    
     destruct st2; try solve [done_right].
     destruct (@H s1); subst; try solve [done_right].
     destruct (@typ_dec t t0); subst; try solve [done_right].
-    destruct (@Size.dec s0 s2); subst; try solve [done_right].
+    destruct (@H0 st2); subst; try solve [done_right].
     destruct (@Align.dec a a0); subst; try solve [auto | done_right].
   Case "sterm_load".    
     destruct st2; try solve [done_right].
@@ -146,7 +146,7 @@ Proof.
     destruct sm2; subst; try solve [done_right].
     destruct (@H sm2); subst; try solve [done_right].
     destruct (@typ_dec t t0); subst; try solve [done_right].
-    destruct (@Size.dec s0 s1); subst; try solve [done_right].
+    destruct (@H0 s1); subst; try solve [done_right].
     destruct (@Align.dec a a0); subst; try solve [auto | done_right].
   Case "smem_free".
     destruct sm2; subst; try solve [done_right].
@@ -157,7 +157,7 @@ Proof.
     destruct sm2; subst; try solve [done_right].
     destruct (@H sm2); subst; try solve [done_right].
     destruct (@typ_dec t t0); subst; try solve [done_right].
-    destruct (@Size.dec s0 s1); subst; try solve [done_right].
+    destruct (@H0 s1); subst; try solve [done_right].
     destruct (@Align.dec a a0); subst; try solve [auto | done_right].
   Case "smem_load".
     destruct sm2; subst; try solve [done_right].
@@ -179,7 +179,7 @@ Proof.
     destruct (@H s2); subst; try solve [done_right].
     destruct (@H0 sf2); subst; try solve [auto | done_right].
     destruct (@typ_dec t t0); subst; try solve [done_right].
-    destruct (@Size.dec s1 s3); subst; try solve [done_right].
+    destruct (@H1 s3); subst; try solve [done_right].
     destruct (@Align.dec a a0); subst; try solve [auto | done_right].
 Qed.
 
